

Programming Language Semantics and Compiler Design

(Sémantique des Langages de Programmation et Compilation)

Structural Operational Semantics of Language **While** and some Extensions

Yliès Falcone

ylies.falcone@univ-grenoble-alpes.fr — www.ylies.fr

Univ. Grenoble Alpes, and LIG-Inria team CORSE

Master of Sciences in Informatics at Grenoble (MoSIG)

Master 1 info

Univ. Grenoble Alpes - UFR IM²AG

www.univ-grenoble-alpes.fr — im2ag.univ-grenoble-alpes.fr

Academic Year 2019 - 2020

Outline - Structural Operational Semantics of Language **While** and some Extensions

Structural Operational Semantics (SOS)

Comparing the Natural and Structural Operational Semantics (NOS vs SOS) of **While**

Comparing NOS and SOS on some Extensions of Language **While**

Conclusion / Summary

Outline - Structural Operational Semantics of Language **While** and some Extensions

Structural Operational Semantics (SOS)

Comparing the Natural and Structural Operational Semantics (NOS vs SOS) of **While**

Comparing NOS and SOS on some Extensions of Language **While**

Conclusion / Summary

Structural Operational Semantics: intuition

Structural Operational Semantics (SOS) is aka “small-step semantics”.

Emphasis on *individual steps* of the execution:

- ▶ tests (of Boolean expression/condition),
- ▶ assignments.

↪ consequences on the definition of computation associated with the other programming constructs.

Intuition on SOS

- ▶ Transitions are of the form:

$$(S, \sigma) \Rightarrow \gamma$$

- ▶ \Rightarrow is the transition relation between configurations.
- ▶ The result γ of an execution step can be either:
 - ▶ (S', σ') : the execution is *not completed*, or
 - ▶ σ' : the execution *has terminated*.

Transition system: natural vs structural semantics

An operational semantics is defined by a **transition system**.

Transition system – general definition (reminder)

A transition system is a 3-tuple (Γ, T, \rightarrow) where:

- ▶ Γ is the set of configurations
- ▶ $T \subseteq \Gamma$ is the set of **final** configurations
- ▶ $\rightarrow \subseteq \Gamma \times \Gamma$ is the transition relation (between configurations)

Transition system for natural operational semantics

1. $\Gamma = (\mathbf{Stm} \times \mathbf{State}) \cup \mathbf{State}$
2. $T = \mathbf{State}$
3. $\rightarrow \subseteq (\mathbf{Stm} \times \mathbf{State}) \times \mathbf{State}$
4. \rightarrow defined by **derivation trees**

Non-final configurations are related (only) to final ones.

Transition system for structural operational semantics

1. $\Gamma = (\mathbf{Stm} \times \mathbf{State}) \cup \mathbf{State}$
2. $T = \mathbf{State}$
3. $\Rightarrow \subseteq (\mathbf{Stm} \times \mathbf{State}) \times ((\mathbf{Stm} \times \mathbf{State}) \cup \mathbf{State})$
4. \Rightarrow defined by **derivation sequences**

Non-final configurations are related to non-final and final ones.

Structural Operational Semantics: Inference System

Goal: Describe how (i.e., step by step) the result of an execution is obtained.

We define \Rightarrow by *induction* on **Stm**.

Axioms

$$\frac{}{(\text{skip}, \sigma) \Rightarrow \sigma} [\text{skip}_{\text{sos}}]$$

$$\frac{}{(x := a, \sigma) \Rightarrow \sigma[x \mapsto \mathcal{A}[a]\sigma]} [\text{ass}_{\text{sos}}]$$

Example 1 (Application of axioms)

- ▶ $(\text{skip}, [x \mapsto 42]) \Rightarrow [x \mapsto 42]$ because $\frac{}{(\text{skip}, [x \mapsto 42]) \Rightarrow [x \mapsto 42]} [\text{skip}_{\text{sos}}]$
- ▶ $(y := 42 + x, [x \mapsto 1]) \Rightarrow \sigma[y \mapsto \mathcal{A}[42 + x][x \mapsto 1]]$

because

$$\frac{}{(y := 42 + x, [x \mapsto 1]) \Rightarrow \sigma[y \mapsto \mathcal{A}[42 + x][x \mapsto 1]]} [\text{ass}_{\text{sos}}]$$

Structural Operational Semantics: Inference System

Rules for sequential statements

$$\frac{(S_1, \sigma) \Rightarrow \sigma'}{(S_1; S_2, \sigma) \Rightarrow (S_2, \sigma')} \text{ [comp}_{\text{sos}}^1]$$

$$\frac{(S_1, \sigma) \Rightarrow (S'_1, \sigma')}{(S_1; S_2, \sigma) \Rightarrow (S'_1; S_2, \sigma')} \text{ [comp}_{\text{sos}}^2]$$

“execution of S_1 has terminated”

“execution of S_1 has not terminated”

Example 2 (Application of the rules for sequential statements)

$$\begin{aligned} ((\text{skip}; x := 42); y := x + 1, []) &\stackrel{(1)}{\Rightarrow} (x := 42; y := x + 1, []) \\ &\stackrel{(2)}{\Rightarrow} (y := x + 1, [x \mapsto 42]) \stackrel{(3)}{\Rightarrow} [x \mapsto 42, y \mapsto 43] \end{aligned}$$

► First derivation ($\stackrel{(1)}{\Rightarrow}$):

$$\frac{\frac{\frac{}{(\text{skip}, []) \Rightarrow []} \text{ [skip}_{\text{sos}}]}}{(\text{skip}; x := 42, []) \Rightarrow (x := 42, [])} \text{ [comp}_{\text{sos}}^1]}{((\text{skip}; x := 42); y := x + 1, []) \Rightarrow (x := 42; y := x + 1, [])} \text{ [comp}_{\text{sos}}^2]$$

► Second derivation ($\stackrel{(2)}{\Rightarrow}$):

$$\frac{\frac{}{(x := 42, []) \Rightarrow [x \mapsto 42]} \text{ [ass}_{\text{sos}}]}}{(x := 42; y := x + 1, []) \Rightarrow (y := x + 1, [x \mapsto 42])} \text{ [comp}_{\text{sos}}^1]$$

► Third derivation ($\stackrel{(3)}{\Rightarrow}$): $\frac{}{(y := x + 1, [x \mapsto 42]) \Rightarrow [x \mapsto 42, y \mapsto 43]} \text{ [ass}_{\text{sos}}]$

Structural Operational Semantics: Inference System (ctd)

Rules for conditional statements

- If $\mathcal{B}[b]\sigma = \mathbf{tt}$, then

$$\frac{}{(\text{if } b \text{ then } S_1 \text{ else } S_2 \text{ fi}, \sigma) \Rightarrow (S_1, \sigma)} [\text{if}_{\text{sos}}^{\mathbf{tt}}]$$

- If $\mathcal{B}[b]\sigma = \mathbf{ff}$, then

$$\frac{}{(\text{if } b \text{ then } S_1 \text{ else } S_2 \text{ fi}, \sigma) \Rightarrow (S_2, \sigma)} [\text{if}_{\text{sos}}^{\mathbf{ff}}]$$

Example 3 (Application of the rules for conditional statements)

$(\text{if } x > 0 \text{ then skip else } x := 42 \text{ fi}, [x \mapsto 0]) \Rightarrow (x := 42, [x \mapsto 0])$

because

$$\frac{}{(\text{if } x > 0 \text{ then skip else } x := 42 \text{ fi}, [x \mapsto 0]) \Rightarrow (x := 42, [x \mapsto 0])} [\text{if}_{\text{sos}}^{\mathbf{ff}}]$$

Rule for iterative statements (unbounded)

$$\frac{}{(\text{while } b \text{ do } S \text{ od}, \sigma) \Rightarrow (\text{if } b \text{ then } (S; \text{while } b \text{ do } S \text{ od}) \text{ else skip fi}, \sigma)} [\text{while}_{\text{sos}}]$$

Exercise 1 (Application of the rule for iterative statements)

Give an example of derivation obtained using the above rule.

Derivation Sequence and Execution

Using the axioms and rules, one can obtain two sorts of derivation sequences.

Definition 1 (Finite derivation sequences)

$$\gamma_1, \gamma_1, \dots, \gamma_k$$

where:

► $\gamma_i \Rightarrow \gamma_{i+1}$, for $i \in [1, k - 1]$, and

► $\gamma_k \not\Rightarrow$

i.e., there is no configuration γ with $\gamma_k \Rightarrow \gamma$

if γ_k is not a final configuration, it is said to be a **blocking configuration**

Definition 2 (Infinite derivation sequences)

$$\gamma_1, \gamma_2, \dots, \text{ where } \gamma_i \Rightarrow \gamma_{i+1}, \text{ for } i \geq 1$$

Definition 3 (Execution of a statement)

The execution(s) of a statement S on a state σ is/are the **maximal** derivation sequence(s) starting with the initial configuration (S, σ) .

Exercise 2 (Derivation sequences)

Give examples of finite and infinite derivation sequences.

The \mathcal{S}_{SOS} semantic function

Definition 4 (The \mathcal{S}_{SOS} semantic function)

$$\mathcal{S}_{\text{SOS}}[S]\sigma = \begin{cases} \sigma' & \text{if } (S, \sigma) \Rightarrow^* \sigma' \\ \text{undef} & \text{otherwise} \end{cases}$$

Example 4 (Applying function \mathcal{S}_{SOS})

- ▶ $\mathcal{S}_{\text{SOS}}[\text{skip}][\sigma] = \sigma$, for any $\sigma \in \mathbf{State}$
- ▶ $\mathcal{S}_{\text{SOS}}[x := 42 + y][y \mapsto 2] = [x \mapsto 44, y \mapsto 42]$
- ▶ $\mathcal{S}_{\text{SOS}}[\text{if } x + y > 0 \text{ then } x := 42 \text{ else } y := 42 \text{ fi}][x \mapsto 1, y \mapsto 2] = [x \mapsto 42, y \mapsto 2]$

Exercise 3 (Applying function \mathcal{S}_{SOS})

Apply function \mathcal{S}_{SOS} to some other statements of your choice in **While**.

Outline - Structural Operational Semantics of Language **While** and some Extensions

Structural Operational Semantics (SOS)

Comparing the Natural and Structural Operational Semantics (NOS vs SOS) of **While**

Comparing NOS and SOS on some Extensions of Language **While**

Conclusion / Summary

Program divergence

How do the two operational semantics model *program divergence*?

Definition 5 (Program divergence)

Consider a statement S and a state σ :

► **Natural semantics:**

S *diverges* in σ , if (S, σ) *does not have a successor (configuration)*:

$$(S, \sigma) \not\rightarrow, \text{ i.e., } \nexists \sigma' \in \mathbf{State} : (S, \sigma) \rightarrow \sigma'$$

(equivalently there exists an infinite derivation tree)

► **Structural semantics:**

S *diverges* in σ ,

if *there exists an infinite derivation sequence* starting from (S, σ) .

(equivalently all configurations have a successor configuration)

Remark As was the case with NOS, there is always at least one derivation of a configuration. In other words, by examining the derivation rules, it is not possible to obtain a stuck configuration. □

Semantic equivalence

Consider two statements S_1 and S_2 .

Semantic equivalence in natural semantics

S_1 and S_2 are **semantically equivalent**, if for all states σ and σ' :

$$(S_1, \sigma) \rightarrow \sigma' \text{ iff } (S_2, \sigma) \rightarrow \sigma'$$

Semantic equivalence in structural semantics

S_1 and S_2 are **semantically equivalent**, if for all states σ

- ▶ for any final or blocking configuration γ :

$$(S_1, \sigma) \Rightarrow^* \gamma \text{ iff } (S_2, \sigma) \Rightarrow^* \gamma$$

- ▶ there exists an infinite derivation sequence starting from (S_1, σ)
iff
there exists an infinite derivation sequence starting from (S_2, σ) .

Equivalence between NOS and SOS?

Do we have $\mathcal{S}_{\text{ns}} = \mathcal{S}_{\text{sos}}$?

(that is, for all $S \in \mathbf{Stm}$, for all $\sigma \in \mathbf{State}$: $\mathcal{S}_{\text{ns}}[S]\sigma = \mathcal{S}_{\text{sos}}[S]\sigma$)

Lemma 1 (NOS “simulates” SOS)

For every statement S in \mathbf{Stm} , states σ and σ' in \mathbf{State} :

$$(S, \sigma) \Rightarrow^k \sigma' \text{ implies } (S, \sigma) \rightarrow \sigma'$$

Lemma 2 (SOS “simulates” NOS)

For every statement S in \mathbf{Stm} , states σ and σ' in \mathbf{State} :

$$(S, \sigma) \rightarrow \sigma' \text{ implies } (S, \sigma) \Rightarrow^* \sigma'$$

Theorem: equivalence of NOS and SOS for **While**

For every statement S in \mathbf{Stm} : $\mathcal{S}_{\text{ns}}[S] = \mathcal{S}_{\text{sos}}[S]$.

Semantic styles and associated proof patterns (reminder)

Inductive semantics: (e.g., functions \mathcal{A}, \mathcal{B})

Construction using composition rules

→ Proofs by structural induction on the (syntax of) the arithmetic/Boolean expressions

Natural operational semantics (“big steps/bird-eye view” of executions)

Transition relation defined by derivation trees.

→ Proofs by induction on the structure of the derivation trees.

Structural operational semantics (“small steps/fine-grain view” of executions)

Transition relation defined by derivation sequences.

→ Proofs by induction on the length of the derivation sequences.

Intermediate Lemma: SOS “simulates” NOS

Lemma 3 (Composing statements)

For every statement $S_1, S_2 \in \mathbf{Stm}$, state $\sigma \in \mathbf{State}$, and $k \in \mathbb{N}$:

$$(S_1, \sigma) \Rightarrow^k \sigma' \text{ implies } (S_1; S_2, \sigma) \Rightarrow^k (S_2; \sigma')$$

(Executing a statement is not influenced by the sequentially composed statement – S_2 in the lemma)

Proof.

By induction on $k \in \mathbb{N}$ (see the tutorial exercises). □

Remark The converse does not hold in general (see the exercises). □

Lemma 4 (SOS “simulates” NOS)

For every statement $S \in \mathbf{Stm}$, states $\sigma, \sigma' \in \mathbf{State}$,

$$(S, \sigma) \rightarrow \sigma' \text{ implies } (S, \sigma) \Rightarrow^* \sigma'.$$

Proof.

By induction on the structure of the derivation tree of $(S, \sigma) \rightarrow \sigma'$. □

Intermediate Lemma: SOS “simulates” NOS

Proof of SOS “simulates” NOS.

By induction on the structure of the derivation tree of $(S, \sigma) \rightarrow \sigma'$. That is, we distinguish cases according to the rule that has been applied to obtain $(S, \sigma) \rightarrow \sigma'$.

[ass_{nos}] S is necessarily a statement of the form $x := a$ (for some $x \in \mathbf{Var}$ and $a \in \mathbf{Aexp}$) and $\sigma' = \sigma[x \mapsto \mathcal{A}[a]\sigma]$ (unique possibility for the rule to be applied). Hence, we have $(x := a, \sigma) \rightarrow \sigma[x \mapsto \mathcal{A}[a]\sigma]$.

Moreover, according to **[ass_{sos}]**, we have $(x := a, \sigma) \Rightarrow \sigma[x \mapsto \mathcal{A}[a]\sigma]$.

[skip_{nos}] Analogous to the previous case.

[comp_{nos}] S is necessarily of the form $S_1; S_2$ and σ' is obtained as follows:

$$\frac{(S_1, \sigma) \rightarrow \sigma'' \quad (S_2, \sigma'') \rightarrow \sigma'}{(S_1; S_2, \sigma) \rightarrow \sigma'}$$

(for some state σ'')

We apply the induction hypothesis to the two premisses $(S_1, \sigma) \rightarrow \sigma''$ and $(S_2, \sigma'') \rightarrow \sigma'$ to obtain $(S_1, \sigma) \Rightarrow^* \sigma''$ and $(S_2, \sigma'') \Rightarrow^* \sigma'$, respectively.

From the lemma (composing statements), we obtain

$(S_1; S_2, \sigma) \Rightarrow^* (S_2, \sigma'')$. And, using $(S_2, \sigma'') \Rightarrow^* \sigma'$ again, we find $(S_1; S_2, \sigma) \Rightarrow^* \sigma'$.



Intermediate Lemma: SOS “simulates” NOS

Proof of SOS “simulates” NOS (ctd).

By induction on the structure of the derivation tree of $(S, \sigma) \rightarrow \sigma'$.

$[if_{nos}^{tt}]$ S is necessarily of the form $\text{if } b \text{ then } S_1 \text{ else } S_2 \text{ fi}$, for some $S_1, S_2 \in \mathbf{Stm}$ and σ' has been obtained as described by the rule:

$$\frac{(S_1, \sigma) \rightarrow \sigma'}{(\text{if } b \text{ then } S_1 \text{ else } S_2 \text{ fi}, \sigma) \rightarrow \sigma'} \quad \mathcal{B}[b]\sigma = \mathbf{tt}$$

Moreover, $(\text{if } b \text{ then } S_1 \text{ else } S_2 \text{ fi}, \sigma) \rightarrow \sigma'$ holds because $\mathcal{B}[b]\sigma = \mathbf{tt}$ and $(S_1, \sigma) \rightarrow \sigma'$.

Since, $\mathcal{B}[b]\sigma = \mathbf{tt}$, we get $(\text{if } b \text{ then } S_1 \text{ else } S_2 \text{ fi}, \sigma) \Rightarrow (S_1, \sigma)$ (because of rule $[if_{sos}^{tt}]$). Moreover, applying the induction hypothesis to the premise $(S_1, \sigma) \rightarrow \sigma'$, we get $(S_1, \sigma) \Rightarrow^* \sigma'$.

From $(S, \sigma) \Rightarrow (S_1, \sigma)$ and $(S_1, \sigma) \Rightarrow^* \sigma'$, we obtain $(S, \sigma) \Rightarrow^* \sigma'$.

$[if_{nos}^{ff}]$ Analogous to $[if_{nos}^{tt}]$.



Intermediate Lemma: SOS “simulates” NOS

Proof of SOS “simulates” NOS (ctd).

By induction on the structure of the derivation tree of $(S, \sigma) \rightarrow \sigma'$.

$[\text{while}_{\text{nos}}^{\text{tt}}]$ We have:

$$\frac{(S', \sigma) \rightarrow \sigma'' \quad (\text{while } b \text{ do } S' \text{ od}, \sigma'') \rightarrow \sigma'}{(\text{while } b \text{ do } S' \text{ od}, \sigma) \rightarrow \sigma'} \quad \mathcal{B}[b]\sigma = \mathbf{tt}$$

That is, we assume that $(\text{while } b \text{ do } S' \text{ od}, \sigma) \rightarrow \sigma'$ holds because $\mathcal{B}[b]\sigma = \mathbf{tt}$, $(S, \sigma) \rightarrow \sigma''$ and $(\text{while } b \text{ do } S' \text{ od}, \sigma'') \rightarrow \sigma'$, for some $S' \in \mathbf{Stm}$, $\sigma'' \in \mathbf{State}$.

The induction hypothesis can be applied to both of the premises $(S', \sigma) \rightarrow \sigma''$ and $(\text{while } b \text{ do } S' \text{ od}, \sigma'') \rightarrow \sigma'$ and gives $(S', \sigma) \Rightarrow^* \sigma''$ and $(\text{while } b \text{ do } S' \text{ od}, \sigma'') \Rightarrow^* \sigma'$.

Using the intermediate lemma (composing statements), we get $(S'; \text{while } b \text{ do } S' \text{ od}, \sigma) \Rightarrow^* \sigma'$. Then, we have the following derivation:

$$\begin{aligned} (\text{while } b \text{ do } S' \text{ od}, \sigma) &\Rightarrow (\text{if } b \text{ then } S'; \text{while } b \text{ do } S' \text{ od else skip fi}, \sigma) && ([\text{while}_{\text{sos}}]) \\ &\Rightarrow (S'; \text{while } b \text{ do } S' \text{ od}, \sigma) && ([\text{if}_{\text{sos}}^{\text{tt}}] \text{ and } \mathcal{B}[b]\sigma = \mathbf{tt}) \\ &\Rightarrow^* \sigma' \end{aligned}$$

$[\text{while}_{\text{nos}}^{\text{tt}}]$ Straightforward.



Intermediate Lemma: NOS “simulates” SOS

We need an additional intermediate lemma.

Lemma 5 (Decomposing computations in SOS)

For every statement $S_1, S_2 \in \mathbf{Stm}$, state $\sigma \in \mathbf{State}$, and $k \in \mathbb{N}$:

$$(S_1; S_2, \sigma) \Rightarrow^k \sigma'' \text{ implies} \\ \text{there exist } \sigma' \text{ and } k_1 \text{ s.t. } (S_1, \sigma) \Rightarrow^{k_1} \sigma' \text{ and } (S_2, \sigma') \Rightarrow^{k-k_1} \sigma''.$$

Proof.

By induction on $k \in \mathbb{N}$ in $(S_1; S_2, \sigma) \Rightarrow^k \sigma''$ (see the tutorial exercises). □

Lemma 6 (NOS “simulates” SOS)

For every statement $S \in \mathbf{Stm}$, state $\sigma \in \mathbf{State}$ and $\sigma' \in \mathbf{State}$, and $k \in \mathbb{N}$:

$$(S, \sigma) \Rightarrow^k \sigma' \text{ implies } (S, \sigma) \rightarrow \sigma'.$$

Proof.

By induction on $k \in \mathbb{N}$ in $(S, \sigma) \Rightarrow^k \sigma'$, i.e., the length of the derivation sequence. □

Intermediate Lemma: NOS “simulates” SOS

NOS “simulates” SOS.

Let us assume that the result holds for all natural numbers lower than or equal to a natural number k and we shall prove the result for $k + 1$. We distinguish how the first step of $(S, \sigma) \Rightarrow^{k+1} \sigma'$ is obtained, that is we inspect the first step of the derivation sequence in the computation in SOS.

[ass_{sos}] Straightforward $((S, \sigma) \Rightarrow^1 \sigma[x \mapsto \mathcal{A}[a]\sigma] \text{ and } k = 0)$.

[skip_{sos}] Straightforward $(S, \sigma) \Rightarrow^1 \sigma, \sigma = \sigma' \text{ and } k = 0)$.

[comp_{sos}^x] Cases [comp_{sos}¹] and [comp_{sos}²]. Necessarily, S is of the form $S_1; S_2$ and we assume that $(S_1; S_2, \sigma) \Rightarrow^{k+1} \sigma''$. We can apply the intermediate lemma to get that there exist $\sigma' \in \mathbf{State}$ and $k_1, k_2 \in \mathbb{N}$ s.t.

$$(S_1, \sigma) \Rightarrow^{k_1} \sigma' \text{ and } (S_2, \sigma') \Rightarrow^{k_2} \sigma''$$

where $k_1 + k_2 = k + 1$. The induction hypothesis can be applied to each of these derivation sequences because $k_1 \leq k$ and $k_2 \leq k$. Hence

$$(S_1, \sigma) \rightarrow \sigma' \text{ and } (S_2, \sigma') \rightarrow \sigma''$$

Using [comp_{nos}], we get $(S_1; S_2, \sigma) \rightarrow \sigma''$.



Intermediate Lemma: NOS “simulates” SOS

NOS “simulates” SOS.

$[if_{\text{SOS}}^{\text{tt}}]$ Assume that $\mathcal{B}[b]\sigma = \text{tt}$ and that

$$(\text{if } b \text{ then } S_1 \text{ else } S_2 \text{ fi}, \sigma) \Rightarrow (S_1, \sigma) \Rightarrow^k \sigma'.$$

The induction hypothesis can be applied to the derivation sequence $(S_1, \sigma) \Rightarrow^k \sigma'$ and gives $(S_1, \sigma) \rightarrow \sigma'$. The result follows using $[if_{\text{NOS}}^{\text{tt}}]$.

$[if_{\text{SOS}}^{\text{ff}}]$ Analogous to the previous case.

$[while_{\text{SOS}}^{\text{tt}}]$ We have:

$$\begin{aligned} (\text{while } b \text{ do } S \text{ od}, \sigma) &\Rightarrow (\text{if } b \text{ then } S; \text{while } b \text{ do } S \text{ od else skip fi}, \sigma) \\ &\Rightarrow^k \sigma'' \end{aligned}$$

The induction hypothesis can be applied to the k last steps of the derivation sequences and gives

$$(\text{if } b \text{ then } S; \text{while } b \text{ do } S \text{ od else skip fi}, \sigma) \rightarrow \sigma''$$

and we get the required $(\text{while } b \text{ do } S \text{ od}, \sigma) \rightarrow \sigma''$ (since $\text{while } b \text{ do } S \text{ od}$ is semantically equivalent to $\text{if } b \text{ then } S; \text{while } b \text{ do } S \text{ od else skip fi}$).



Outline - Structural Operational Semantics of Language **While** and some Extensions

Structural Operational Semantics (SOS)

Comparing the Natural and Structural Operational Semantics (NOS vs SOS) of **While**

Comparing NOS and SOS on some Extensions of Language **While**

Command **abort** for abnormal termination

Operator **or** for Non-Determinism

The **||** Operator for Parallelism

Conclusion / Summary

Outline - Structural Operational Semantics of Language **While** and some Extensions

Structural Operational Semantics (SOS)

Comparing the Natural and Structural Operational Semantics (NOS vs SOS) of **While**

Comparing NOS and SOS on some Extensions of Language **While**

Command **abort** for abnormal termination

Operator **or** for Non-Determinism

The **||** Operator for Parallelism

Conclusion / Summary

Extending **While** with abnormal termination

Definition 6 (Introducing statement **abort**)

- ▶ Statement **abort**: used to represent abnormal terminating computations
- ▶ “Behaves” differently than previous statements:
 - ↪ It stops the program
 - ▶ different from **while true do skip od**, and
 - ▶ different from **skip**.
- ▶ Configuration (abort, σ) has no successors (blocking):

for all $\sigma \in \mathbf{State}$: $(\text{abort}, \sigma) \nrightarrow$ (in NOS)
 and
 for all $\sigma \in \mathbf{State}$: $(\text{abort}, \sigma) \nRightarrow$ (in SOS)

↪ we *do not* add any rule to the transitions systems

Example 5 (Program with possible abnormal termination)

```
var sensor := some initial value
...
sensor := read(...)
if sensor < 0 then abort else skip fi
```

Examples with abort

Exercise 4 (Assertions)

Using the abort construct, provide natural and structural operational semantics rules to the following construct:

assert b before S

The informal semantics is that one should check that b holds before executing S. If b does not hold, S should not be executed.

Comparison of **abort** in natural and structural semantics

In *natural* operational semantics:

- ▶ abort, and
- ▶ while true do skip od,

are semantically equivalent.

In *natural* operational semantics:

- ▶ abort, and
- ▶ skip,

are not semantically equivalent.

In *structural* operational semantics:

- ▶ while true do skip od,
- ▶ abort, and
- ▶ skip,

are pair-wise not semantically equivalent.

Outline - Structural Operational Semantics of Language **While** and some Extensions

Structural Operational Semantics (SOS)

Comparing the Natural and Structural Operational Semantics (NOS vs SOS) of **While**

Comparing NOS and SOS on some Extensions of Language **While**

Command **abort** for abnormal termination

Operator **or** for Non-Determinism

The **||** Operator for Parallelism

Conclusion / Summary

Operator **or**

Definition 7 (Or operator)

- ▶ Non-determinism
- ▶ Statement S_1 or S_2

We note the new obtained language **While**^{or}

Example 6 (Using the or operator)

We expect that the execution of the statement

$$x := 1 \quad \text{or} \quad x := 2$$

could result in a state where x has the value 1 or 2.

The **or** operator: extending the transition system

Definition 8 (NOS and SOS transition systems for operator **or**)

► Configurations: $(\mathbf{While}^{\text{or}} \times \mathbf{State}) \cup \mathbf{State}$

► Natural semantics:

$$\frac{(S_1, \sigma) \rightarrow \sigma'}{(S_1 \text{ or } S_2, \sigma) \rightarrow \sigma'}$$

$$\frac{(S_2, \sigma) \rightarrow \sigma'}{(S_1 \text{ or } S_2, \sigma) \rightarrow \sigma'}$$

► Structural semantics:

$$(S_1 \text{ or } S_2, \sigma) \Rightarrow (S_1, \sigma)$$

$$(S_1 \text{ or } S_2, \sigma) \Rightarrow (S_2, \sigma)$$

Example 7 (Applying the rules of operator **or**)

Consider the statement $x := 1 \text{ or } x := 2$.

► Natural semantics:

$$\frac{\overline{(x := 1, []) \rightarrow [x \mapsto 1]}}{(x := 1 \text{ or } x := 2, []) \rightarrow [x \mapsto 1]} \quad \frac{\overline{(x := 2, []) \rightarrow [x \mapsto 2]}}{(x := 1 \text{ or } x := 2, []) \rightarrow [x \mapsto 2]}$$

► Structural semantics:

$$\begin{aligned} (x := 1 \text{ or } x := 2, []) &\Rightarrow (x := 1, []) \Rightarrow [x \mapsto 1] \\ (x := 1 \text{ or } x := 2, []) &\Rightarrow (x := 2, []) \Rightarrow [x \mapsto 2] \end{aligned}$$

Discussion on **or** and non-termination

With natural operational semantics, operator **or** **hides non-termination**.

Example 8 (**or** and non-termination in NOS and SOS)

Consider the two following statements:

- ▶ $S_1 = \text{while true do skip od}$
- ▶ $S_2 = \text{while false do skip od}$

Comparing semantics:

- ▶ natural semantics: $(S_1 \text{ or } S_2, \sigma)$ has one derivation tree (the one corresponding to S_2);
- ▶ structural semantics: $(S_1 \text{ or } S_2)$ has an infinite derivation sequence for S_1 (in addition to the finite one for S_2).

Henceforth:

- ▶ in NOS: $S_1 \text{ or } S_2$ and S_2 are semantically equivalent;
- ▶ in SOS: $S_1 \text{ or } S_2$, S_1 , and S_2 are *pairwise not* semantically equivalent.

Natural/structural operational semantics and looping

- ▶ In NOS, non-determinism “hides” looping, if possible.
- ▶ In SOS, non-determinism does not “hide” looping.

Outline - Structural Operational Semantics of Language **While** and some Extensions

Structural Operational Semantics (SOS)

Comparing the Natural and Structural Operational Semantics (NOS vs SOS) of **While**

Comparing NOS and SOS on some Extensions of Language **While**

Command **abort** for abnormal termination

Operator **or** for Non-Determinism

The **||** Operator for Parallelism

Conclusion / Summary

Parallel execution

We add a construct noted \parallel (syntactic extension).

In $S_1 \parallel S_2$, we expect S_1 and S_2 to execute in parallel (informal semantics).

We refer to this new language as **While** ^{\parallel} .

Definition 9 (Extending the transition system for parallel execution)

- ▶ Configurations: $(\text{While}^{\parallel} \times \text{State}) \cup \text{State}$.
- ▶ Additional transition rules to handle \parallel :

- ▶ **Natural semantics:**

$$\frac{(S_1, \sigma) \rightarrow \sigma' \quad (S_2, \sigma') \rightarrow \sigma''}{(S_1 \parallel S_2, \sigma) \rightarrow \sigma''} \quad \frac{(S_2, \sigma) \rightarrow \sigma' \quad (S_1, \sigma') \rightarrow \sigma''}{(S_1 \parallel S_2, \sigma) \rightarrow \sigma''}$$

→ The executions of immediate constituents (S_1 and S_2) are *atomic*.

- ▶ **Structural semantics:**

$$\frac{(S_1, \sigma) \Rightarrow (S'_1, \sigma')}{(S_1 \parallel S_2, \sigma) \Rightarrow (S'_1 \parallel S_2, \sigma')} \quad \frac{(S_2, \sigma) \Rightarrow (S'_2, \sigma')}{(S_1 \parallel S_2, \sigma) \Rightarrow (S_1 \parallel S'_2, \sigma')}$$

$$\frac{(S_1, \sigma) \Rightarrow \sigma'}{(S_1 \parallel S_2, \sigma) \Rightarrow (S_2, \sigma')} \quad \frac{(S_2, \sigma) \Rightarrow \sigma'}{(S_1 \parallel S_2, \sigma) \Rightarrow (S_1, \sigma')}$$

→ The executions of immediate constituents (S_1 and S_2) are *interleaved*.

Discussion about the parallelism and interleaving

Example 9 (Parallel execution)

Consider the following statement:

$$x := 1 \parallel (x := 2; x := x + 2)$$

- ▶ **natural operational semantics**: 2 possible ending states
- ▶ **structural operational semantics**: 3 possible ending states

Exercise 5 (Applying the rules for parallel execution)

Apply the new semantic rules to the statement in the previous example to determine the possible resulting states.

Natural vs Structural (operational) semantics and interleaving

- ▶ **Natural semantics**:
 - ▶ does not allow to express **interleaving**
 - ▶ executions of atomic constituents are atomic
- ▶ **Structural semantics**:
 - ▶ allows to express **interleaving**
 - ▶ we focus on the small steps of computations

Outline - Structural Operational Semantics of Language **While** and some Extensions

Structural Operational Semantics (SOS)

Comparing the Natural and Structural Operational Semantics (NOS vs SOS) of **While**

Comparing NOS and SOS on some Extensions of Language **While**

Conclusion / Summary

Conclusion / Summary: Structural Operational Semantics of Language **While** and some Extensions

Natural operational semantics (NOS):

- ▶ bird-eye view of computations
- ▶ does not distinguish between blocking and non-termination,
- ▶ non-determinism “hides” non-termination,
- ▶ does not allow to express an interleaving semantics.

Structural operational semantics (SOS):

- ▶ step-by-step view of execution (sequential composition, evaluation of conditions)
- ▶ distinguishes between blocking and non-termination,
- ▶ non-determinism does not “hide” non-termination,
- ▶ allows to express an interleaving semantics.

NOS and SOS are equivalent for **While** and not equivalent for the studied extensions.